WIP

ems/LSimModSem.v
@@ -1233,7 +1233,7 @@ Proof.
     eapply incl_appr; ss.
 Qed.
 
-Require Import SimGlobal.
+Require Import GSimModSem.
 
 Module TAC.
   Ltac ired_l := try (prw _red_gen 2 0).
@@ -1318,16 +1318,16 @@ Unshelve.
   esplits; et.
 Qed.
 
-Theorem adequacy
+Theorem adequacy_whole
   `{EMSConfig}
   (P Q: Prop)
   ms_src ms_tgt
   (SIM: ModSemPair.sim ms_src ms_tgt)
   (WF: P -> Q)
   :
-  (Beh.of_program (ModSem.compile ms_tgt (Some P)))
+  (Beh.of_program (ModSem.compile ms_tgt P))
   <1=
-    (Beh.of_program (ModSem.compile ms_src (Some Q))).
+    (Beh.of_program (ModSem.compile ms_src Q)).
 Proof.
   eapply adequacy_global_itree; ss.
   inv SIM.
@@ -1346,136 +1346,17 @@ Proof.
   { i. des_ifs. r in SIM0. des; clarify. steps. }
 Qed.
 
-End ModSemPair.
-
-
-
-
-
-
-
-
-Module ModPair.
-Section SIMMOD.
-  Context `{LD: Sk.ld}.
-  Variable (md_src md_tgt: Mod.t).
-  Inductive sim: Prop := mk {
-    sim_modsem:
-      forall sk_src sk_tgt
-             (EXT: Sk.extends sk_src sk_tgt)
-             (SKWF: Sk.wf (sk_tgt ⊕ md_tgt.(Mod.sk))),
-        <<SIM: ModSemPair.sim (md_src.(Mod.get_modsem) (sk_src ⊕ md_src.(Mod.sk)))
-                 (md_tgt.(Mod.get_modsem) (sk_tgt ⊕ md_tgt.(Mod.sk)))>>;
-    sim_sk: Sk.extends md_src.(Mod.sk) md_tgt.(Mod.sk);
-  }.
-
-End SIMMOD.
-
-Section FACTS.
-
-Context `{LD: Sk.ld}.
-
-Theorem compose
-  md_src0 md_tgt0 md_src1 md_tgt1
-  (SIM0: ModPair.sim md_src0 md_tgt0)
-  (SIM1: ModPair.sim md_src1 md_tgt1)
-  :
-  <<SIM: ModPair.sim (md_src0 ⊕ md_src1) (md_tgt0 ⊕ md_tgt1)>>
-.
-Proof.
-  inv SIM0.
-  inv SIM1.
-  des.
-  econs; ss.
-  2:{ i. rewrite sim_sk0. rewrite sim_sk1. refl. }
-  ii; ss.
-  eapply ModSemPair.compose; et.
-  - assert(T: sk_src ⊕ (Mod.sk md_src0 ⊕ Mod.sk md_src1) ≡ (sk_src ⊕ Mod.sk md_src1) ⊕ Mod.sk md_src0).
-    { rewrite <- ! Sk.add_assoc. eapply Sk.add_equiv; try refl. eapply Sk.add_comm; et. }
-    erewrite (Mod.get_modsem_Proper md_src0); try eapply T.
-    2: { eapply Sk.wf_mon; et. rewrite sim_sk0. rewrite sim_sk1. rewrite EXT. refl. }
-    assert(U: sk_tgt ⊕ (Mod.sk md_tgt0 ⊕ Mod.sk md_tgt1) ≡ (sk_tgt ⊕ Mod.sk md_tgt1) ⊕ Mod.sk md_tgt0).
-    { rewrite <- ! Sk.add_assoc. eapply Sk.add_equiv; try refl. eapply Sk.add_comm; et. }
-    erewrite (Mod.get_modsem_Proper md_tgt0); try eapply U.
-    2: { ss. }
-    eapply sim_modsem0; ss.
-    2: { rewrite <- U; et. }
-    rewrite EXT. rewrite sim_sk1. refl.
-  - assert(T: sk_src ⊕ (Mod.sk md_src0 ⊕ Mod.sk md_src1) ≡ (sk_src ⊕ Mod.sk md_src0) ⊕ Mod.sk md_src1).
-    { rewrite <- ! Sk.add_assoc. eapply Sk.add_equiv; try refl. }
-    erewrite (Mod.get_modsem_Proper md_src1); try eapply T.
-    2: { eapply Sk.wf_mon; et. rewrite sim_sk0. rewrite sim_sk1. rewrite EXT. refl. }
-    assert(U: sk_tgt ⊕ (Mod.sk md_tgt0 ⊕ Mod.sk md_tgt1) ≡ (sk_tgt ⊕ Mod.sk md_tgt0) ⊕ Mod.sk md_tgt1).
-    { rewrite <- ! Sk.add_assoc. eapply Sk.add_equiv; try refl. }
-    erewrite (Mod.get_modsem_Proper md_tgt1); try eapply U.
-    2: { ss. }
-    eapply sim_modsem1; ss.
-    2: { rewrite <- U; et. }
-    rewrite EXT. rewrite sim_sk0. refl.
-Qed.
-
 Theorem adequacy
-  md_src md_tgt
-  (SIM: ModPair.sim md_src md_tgt)
+  ms_src ms_tgt
+  (SIM: ModSemPair.sim ms_src ms_tgt)
   :
-  md_tgt ⊑ md_src
+  ms_tgt ⊑ ms_src
 .
 Proof.
-  ii. unfold Mod.compile, Mod.enclose in *.
-  destruct (classic (Mod.wf (ctx ⊕ md_tgt))).
-  2:{ eapply ModSem.compile_not_wf in PR; ss. subst. eapply Beh.nb_bottom. }
-  pose (sk_tgt := (Mod.sk (ctx ⊕ md_tgt))).
-  pose (sk_src := (Mod.sk (ctx ⊕ md_src))).
-  destruct (classic (Sk.wf (Mod.sk md_tgt))); rename H0 into SKWF.
-  2: { eapply ModSem.initial_itr_not_wf in PR; ss.
-       { subst. eapply Beh.nb_bottom. }
-       intro T. eapply SKWF. inv T; ss. eapply Sk.wf_mon; et. r. esplits; et.
-       rewrite Sk.add_comm; et. refl. }
-  (* assert (SKEQ: sk_tgt ≡ sk_src). *)
-  (* { unfold sk_src, sk_tgt. ss. inv SIM. spc sim_sk0. rewrite sim_sk0. refl. } *)
-  assert(EXT: Sk.extends sk_src sk_tgt).
-  { subst sk_src sk_tgt. ss. inv SIM. rewrite sim_sk0. refl. }
-
-  rr in H. unfold Mod.enclose in *. fold sk_src in H. des. inv WF.
-  {
-    folder.
-    inv SIM. ss.
-    exploit sim_modsem0.
-    { refl. }
-    { eauto. }
-    intro T; des.
-    eapply ModSemPair.adequacy; revgoals; et.
-    2: {
-      eapply ModSemPair.compose.
-      - erewrite <- Mod.get_modsem_Proper; et; try by (eapply Sk.wf_equiv; [sym; et|]; ss).
-      - eapply ModSemPair.self_sim.
-      - eapply sim_modsem0; et.
-        { r. subst sk_tgt. esplits. rewrite Sk.add_comm; refl. }
-        rewrite SKEQ; ss.
-    }
-    { unfold Mod.wf, Mod.enclose. ii. ss. des; ss. folder. esplits; et.
-      2: { rewrite SKEQ; ss. }
-      {
-        erewrite Mod.get_modsem_Proper; et; try by (eapply Sk.wf_equiv; [sym; et|]; ss).
-        rewrite (Mod.get_modsem_Proper _ _ _ SKEQ); et; try by (eapply Sk.wf_equiv; [sym; et|]; ss).
-        econs.
-      }
-    }
-  }
+  ii.
+  eapply adequacy_whole; et.
+  eapply compose; et. eapply self_sim.
 Qed.
 
-Corollary adequacy'
-  `{EMSConfig}
-  md_src md_tgt
-  (SIM: ModPair.sim md_src md_tgt)
-  :
-  md_tgt ⊑ md_src
-.
-Proof.
-  eapply adequacy; ss.
-Qed.
-
-End FACTS.
-End ModPair.
-
+End ModSemPair.
 
