ems/GSimMod.v
@@ -1,0 +1,29 @@
+Require Import Coqlib.
+Require Import ITreelib.
+Require Import Any.
+Require Import STS.
+Require Import Behavior.
+Require Import Mod ModSem.
+Require Import Skeleton.
+Require Import Coq.Relations.Relation_Definitions.
+Require Import Relation_Operators.
+Require Import RelationPairs.
+From Ordinal Require Import Ordinal Arithmetic.
+Require Import SimSTS SimModSemGlobal.
+
+Set Implicit Arguments.
+
+
+Variable md_src md_tgt: Mod.t.
+Let ms_src: ModSem.t := md_src.(Mod.enclose).
+Let ms_tgt: ModSem.t := md_tgt.(Mod.enclose).
+
+Section ADEQUACY.
+Hypothesis (SIM: simg eq false false (@ModSem.initial_itr ms_src CONFS (Some (Mod.wf md_src))) (@ModSem.initial_itr ms_tgt CONFT (Some (Mod.wf md_tgt)))).
+
+
+Theorem adequacy_global: Beh.of_program (@Mod.compile _ CONFT md_tgt) <1= Beh.of_program (@Mod.compile _ CONFS md_src).
+Proof.
+  eapply adequacy_global_itree. eapply SIM.
+Qed.
+End ADEQUACY.
