ems/GSimModSem.v
@@ -684,20 +684,6 @@ Proof.
   { gstep. eapply sim_progress; eauto. gbase. auto. }
 Qed.
 
-
-Variable md_src md_tgt: Mod.t.
-Let ms_src: ModSem.t := md_src.(Mod.enclose).
-Let ms_tgt: ModSem.t := md_tgt.(Mod.enclose).
-
-Section ADEQUACY.
-Hypothesis (SIM: simg eq false false (@ModSem.initial_itr ms_src CONFS (Some (Mod.wf md_src))) (@ModSem.initial_itr ms_tgt CONFT (Some (Mod.wf md_tgt)))).
-
-
-Theorem adequacy_global: Beh.of_program (@Mod.compile _ CONFT md_tgt) <1= Beh.of_program (@Mod.compile _ CONFS md_src).
-Proof.
-  eapply adequacy_global_itree. eapply SIM.
-Qed.
-End ADEQUACY.
 End SIM.
 
 Hint Constructors _simg.
