ems/Mod.v
@@ -1,0 +1,127 @@
+Require Import Coqlib.
+Require Export sflib.
+Require Export ITreelib.
+Require Export ModSem ModSemE.
+Export Events.
+Require Export AList.
+Require Import Skeleton.
+Require Import STS Behavior.
+Require Import Any.
+Require Import Permutation.
+
+Set Implicit Arguments.
+
+
+Module Mod.
+Section MOD.
+  Context `{Sk.ld}.
+
+  Record t: Type := mk {
+    get_modsem: Sk.t -> ModSem.t;
+    sk: Sk.t;
+    enclose: ModSem.t := (get_modsem sk);
+    (* get_modsem_Proper:> Proper ((≡) ==> eq) get_modsem; *)
+    get_modsem_Proper:> forall sk0 sk1 (EQV: sk0 ≡ sk1) (WF: Sk.wf sk0), get_modsem sk0 = get_modsem sk1;
+    get_modsem_extends:> forall sk0 sk1 (EQV: Sk.extends sk0 sk1) (WF: Sk.wf sk1), get_modsem sk1 ⊑ get_modsem sk0;
+    get_modsem_extends_core:> forall sk0 sk1 (EQV: Sk.extends sk0 sk1) (WF: Sk.wf sk1), | get_modsem sk1 | ⊑ | get_modsem sk0 |;
+  }
+  .
+
+  (* Definition wf (md: t): Prop := (<<SK: Sk.wf (md.(sk))>>). *)
+  Definition wf (md: t): Prop := (<<WF: ModSem.wf md.(enclose)>> /\ <<SK: Sk.wf (md.(sk))>>).
+
+  Program Definition core (md: t): t := mk (fun sk => |(md.(get_modsem) sk)| ) md.(sk) _ _ _.
+  Next Obligation.
+    erewrite get_modsem_Proper; et.
+  Qed.
+  Next Obligation.
+    eapply get_modsem_extends_core; et.
+  Qed.
+  Next Obligation.
+    rewrite ! ModSem.core_idemp.
+    eapply get_modsem_extends_core; et.
+  Qed.
+
+  Global Program Instance bar: Bar t := core.
+
+  Section BEH.
+
+  Context {CONF: EMSConfig}.
+
+  Definition compile (md: t): semantics :=
+    ModSem.compile_itree (ModSem.initial_itr md.(enclose) (Some (wf md))).
+
+  (* Record wf (md: t): Prop := mk_wf { *)
+  (*   wf_sk: Sk.wf md.(sk); *)
+  (* } *)
+  (* . *)
+  (*** wf about modsem is enforced in the semantics ***)
+
+  Program Definition add (md0 md1: t): t := {|
+    get_modsem := fun sk => (md0.(get_modsem) sk) ⊕ (md1.(get_modsem) sk);
+    sk := md0.(sk) ⊕ md1.(sk);
+  |}
+  .
+  Next Obligation.
+    ii. rewrite ! (@get_modsem_Proper _ _ _ EQV); et.
+  Qed.
+  Next Obligation.
+    admit "should hold".
+  Qed.
+  Next Obligation.
+    admit "should hold".
+  Qed.
+
+  Global Program Instance add_OPlus: OPlus t := add.
+
+  Program Definition empty: t := {|
+    get_modsem := fun _ => ModSem.mk [] tt↑;
+    sk := Sk.unit;
+  |}
+  .
+  Next Obligation.
+    ss.
+  Qed.
+  Next Obligation.
+    ss.
+  Qed.
+
+  End BEH.
+
+  Section REFINE.
+
+  Definition cref' {CONF: EMSConfig} (md_tgt md_src: t): Prop :=
+    forall (ctx: t), Beh.of_program (compile (ctx ⊕ md_tgt)) <1=
+                       Beh.of_program (compile (ctx ⊕ md_src))
+  .
+
+  Definition cref (md_tgt md_src: t): Prop :=
+    forall {CONF: EMSConfig}, cref' md_tgt md_src.
+
+  Section CONF.
+    Context {CONF: EMSConfig}.
+
+    Global Program Instance cref_PreOrder: PreOrder cref.
+    Next Obligation.
+      ii. ss.
+    Qed.
+    Next Obligation.
+      ii. eapply H0 in PR. eapply H1 in PR. eapply PR.
+    Qed.
+
+    Global Program Instance cref'_PreOrder: PreOrder cref'.
+    Next Obligation. ii. ss. Qed.
+    Next Obligation. ii. eapply H1. eapply H0. ss. Qed.
+  End CONF.
+
+  Definition bref {CONF: EMSConfig} (md_tgt md_src: t): Prop :=
+    Beh.of_program (compile md_tgt) <1= Beh.of_program (compile md_src)
+  .
+
+  End REFINE.
+
+End MOD.
+End Mod.
+
+Notation "(⊑B)" := Mod.bref (at level 50).
+Notation "a ⊑B b" := (Mod.bref a b) (at level 50).
