ems/ModSemFacts.v
@@ -1,0 +1,111 @@
+Require Import Coqlib.
+Require Export sflib.
+Require Export ITreelib.
+Require Export ModSemE.
+Require Export AList.
+Require Import Skeleton.
+Require Import STS Behavior.
+Require Import Any.
+Require Import Permutation.
+Require Import ModSem.
+Require Import LSimModSem.
+
+Set Implicit Arguments.
+
+
+Section FACTS.
+
+Global Program Instance ModSem_OPlusFactsWeak: OPlusFactsWeak (T:=ModSem.t).
+Next Obligation.
+  eapply ModSemPair.adequacy.
+  econs.
+  { instantiate (1:=top2). ss. }
+  2: { instantiate (2:=unit).
+       instantiate (1:=fun _ '(st_src, st_tgt) => exists st0 st1, st_tgt = Any.pair st0 st1 /\ st_src = Any.pair st1 st0).
+       ss. esplits; et. ss. }
+  i. ss. rewrite in_app_iff in FINDS. des.
+  - rewrite in_map_iff in *. des; ss. destruct x; ss. clarify.
+    esplits; et.
+    { rewrite in_app_iff. right. rewrite in_map_iff. esplits; et. ss. }
+    admit "ez".
+  - rewrite in_map_iff in *. des; ss. destruct x; ss. clarify.
+    esplits; et.
+    { rewrite in_app_iff. left. rewrite in_map_iff. esplits; et. ss. }
+    admit "ez".
+    Unshelve.
+Qed.
+Next Obligation.
+  eapply ModSemPair.adequacy.
+  econs; eauto.
+  { instantiate (1:=top2). ss. }
+  2: { instantiate (2:=unit).
+       instantiate (1:=fun _ '(st_src, st_tgt) => exists st0 st1 st2,
+                           st_tgt = (Any.pair st0 (Any.pair st1 st2)) /\ st_src = (Any.pair (Any.pair st0 st1) st2)).
+       ss. esplits; et. ss. }
+  i. ss. rewrite in_app_iff in FINDS. des.
+  2: {
+    rewrite in_map_iff in *. des; ss. destruct x; ss. clarify.
+    esplits; et.
+    { rewrite in_app_iff. right. rewrite in_map_iff. eexists (_, _); ss. esplits; et. rewrite in_app_iff. right; ss.
+      rewrite in_map_iff. esplits; et. ss.
+    }
+    admit "ez".
+  }
+  rewrite in_map_iff in *. des. destruct x; ss; clarify. rewrite in_app_iff in *. des.
+  {
+    rewrite in_map_iff in *. des; ss. destruct x; ss. clarify.
+    esplits; et.
+    { rewrite in_app_iff. left. rewrite in_map_iff. esplits; et. ss.
+    }
+    admit "ez".
+  }
+  {
+    rewrite in_map_iff in *. des; ss. destruct x; ss. clarify.
+    esplits; et.
+    { rewrite in_app_iff. right. rewrite in_map_iff. eexists (_, _); ss. esplits; et. rewrite in_app_iff. left; ss.
+      rewrite in_map_iff. esplits; et. ss.
+    }
+    admit "ez".
+  }
+Qed.
+Next Obligation.
+  ii. rr in H. des. rr in H0. des. rr. ss. esplits; et.
+  2: { congruence. }
+  eapply Forall2_app.
+  - eapply Forall2_apply_Forall2; et. ii; ss. des_ifs. ss. des; clarify. esplits; et.
+    ii. unfold focus_left. rewrite H4. refl.
+  - eapply Forall2_apply_Forall2; et. ii; ss. des_ifs. ss. des; clarify. esplits; et.
+    ii. unfold focus_right. rewrite H4. refl.
+Qed.
+
+Global Program Instance ModSem_Ref_PreOrder: PreOrder ((⊑)).
+Next Obligation.
+  ii; ss.
+Qed.
+Next Obligation.
+  ii. eapply H0. eapply H; ss.
+Qed.
+
+Global Program Instance ModSem_EpsFacts: EpsFacts.
+Next Obligation.
+  ii; ss.
+Qed.
+Next Obligation.
+  ii. eapply H0. eapply H; ss.
+Qed.
+
+Global Program Instance ModSem_RefFacts: RefFacts (T:=ModSem.t).
+Next Obligation.
+  do 3 r. i.
+  {
+    ii.
+    eapply oplus_assoc_weak.
+  }
+  
+  rewrite oplus_assoc_weak.
+  rewrite H.
+  - ii; ss.
+  - ii. eapply H0. eapply H; ss.
+Qed.
+
+End FACTS.
